Clean proofs a bit.

src/Eval/Prog.v
@@ -145,28 +145,36 @@ Fixpoint split_expr (e : expr) (lp lc : list expr) :=
     end
   end.
 
-Lemma eval_nth_rcons_unique : forall vars e l, eval e vars = eval e nil -> (
-  forall n, eval (nth n l (Econst (Int 0))) vars = eval (nth n l (Econst (Int 0))) nil) ->
-    forall n,
-    eval (nth n (rcons_unique e l) (Econst (Int 0))) vars = eval (nth n (rcons_unique e l) (Econst (Int 0))) nil.
+Lemma eval_nth_rcons_unique :
+  forall d vars vars' e l,
+  eval e vars = eval e vars' ->
+  (forall n, eval (nth n l d) vars = eval (nth n l d) vars') ->
+  forall n,
+  eval (nth n (rcons_unique e l) d) vars = eval (nth n (rcons_unique e l) d) vars'.
 Proof.
-intros vars e l He Hl. induction l as [|h t IH] ; simpl; [now intros [|[|n]] |].
-generalize (internal_expr_dec_bl e h). destruct expr_beq.
-intros H [|n]. simpl. now rewrite <- H.
-apply Hl. intros _ [|n]. apply (Hl 0%nat). apply IH. intros n'.
+intros d vars vars' e l He Hl.
+induction l as [|h t IH] ; simpl.
+{ simpl in Hl. now intros [|n]. }
+generalize (internal_expr_dec_bl e h).
+destruct expr_beq.
+{ now intros _. }
+intros _ [|n].
+{ apply (Hl 0). }
+apply IH.
+intros n'.
 apply (Hl (S n')).
 Qed.
 
 Theorem split_expr_correct :
-  forall vars e lp lc,
-  (forall n, eval (nth n lc (Econst (Int 0))) vars = eval (nth n lc (Econst (Int 0))) nil) ->
+  forall d vars vars' e lp lc,
+  (forall n, eval (nth n lc d) vars = eval (nth n lc d) vars') ->
   match split_expr e lp lc with
-  | Sconst => eval e vars = eval e nil
+  | Sconst => eval e vars = eval e vars'
   | Scomposed lp' lc' =>
-    forall n, eval (nth n lc' (Econst (Int 0))) vars = eval (nth n lc' (Econst (Int 0))) nil
+    forall n, eval (nth n lc' d) vars = eval (nth n lc' d) vars'
   end.
 Proof.
-intros vars.
+intros d vars vars'.
 induction e as [n|o|o e1 IHe1|o e1 IHe1 e2 IHe2] ; intros lp lc Hc ; simpl ; try easy.
   specialize (IHe1 lp lc Hc).
   destruct split_expr as [|lp' lc'].
@@ -401,43 +409,57 @@ Fixpoint max_arity (e : expr) (n : nat) :=
   | Ebinary o e1 e2 => if max_arity e1 n then max_arity e2 n else false
   end.
 
-Lemma max_arity_correct : forall e k, max_arity e k = true ->
-  forall vars v, k <= length vars ->
+Lemma max_arity_correct :
+  forall e vars v,
+  max_arity e (length vars) = true ->
   eval e (vars ++ v) = eval e vars.
 Proof.
-induction e as [n | o | o e | o e1 e2]; [ | easy | | ]; simpl in *; intros k.
-- rewrite Nat.ltb_lt. intros Hnk vars v Hk.
-  apply Nat.lt_le_trans with (1 := Hnk) in Hk. now apply app_nth1.
-- intros Hek vars v Hk. now rewrite (IHe k).
-- rewrite <-Bool.andb_lazy_alt. intros H vars v Hk.
-  apply andb_prop in H. destruct H as [H1 H3].
-  now rewrite (e2 k), (IHe1 k).
+induction e as [n|o|o e IH|o e1 IH1 e2 IH2] ; simpl ; intros vars v H.
+- apply app_nth1.
+  now apply Nat.ltb_lt.
+- easy.
+- now rewrite IH.
+- rewrite <- Bool.andb_lazy_alt in H.
+  apply andb_prop in H.
+  rewrite IH1 by easy.
+  now rewrite IH2.
 Qed.
 
 Inductive extracted_expr : Set :=
   | Eabort
   | Eprog (lp : list term) (lc : list expr).
 
-Fixpoint fold_split (le lp lc : list expr) := match le with
-  | nil     => (lp, lc)
-  | e :: le => let (lp, lc) := fold_split le lp lc in
+Fixpoint fold_split (le lp lc : list expr) :=
+  match le with
+  | nil => (lp, lc)
+  | e :: le =>
+    let (lp, lc) := fold_split le lp lc in
     match split_expr e lp lc with
     | Sconst => (lp, (rcons_unique e lc))
     | Scomposed lp lc => (lp, lc)
     end
   end.
 
-Fixpoint max_arity_list (le : list expr) (vars : nat) := match le with
+Fixpoint max_arity_list (le : list expr) (vars : nat) :=
+  match le with
   | nil => true
-  | e :: le => andb (max_arity e vars) (max_arity_list le vars) end.
+  | e :: le => andb (max_arity e vars) (max_arity_list le vars)
+  end.
 
-Lemma max_arity_nth : forall le vars k d, max_arity_list le vars = true ->
-  k < length le -> max_arity (nth k le d) vars = true.
+Lemma max_arity_nth :
+  forall le vars k d,
+  max_arity_list le vars = true ->
+  k < length le ->
+  max_arity (nth k le d) vars = true.
 Proof.
-induction le; [easy | ].
-intros vars [ | k] d H Hk; simpl in *; apply andb_prop in H; destruct H as [Ha Hle];
-  [assumption |].
-apply lt_S_n in Hk. now apply IHle.
+induction le ; try easy.
+intros vars k d H Hk.
+simpl in H.
+apply andb_prop in H.
+destruct H as [Ha Hle].
+destruct k as [|k] ; try easy.
+apply IHle with (1 := Hle).
+now apply lt_S_n in Hk.
 Qed.
 
 Definition extract_list (le : list expr) (vars : nat) :=
@@ -462,11 +484,10 @@ Theorem extract_list_correct :
 Proof.
 intros le vars.
 unfold extract_list.
-destruct max_arity_list eqn:Ha; [ | exact I].
+destruct max_arity_list eqn:Ha ; [ |exact I].
 destruct fold_split as (lp, lc) eqn:Hf.
-destruct decompose as [lp' | ] eqn:Hd; [ | easy].
-
-generalize (decompose_correct vars nil (le ++ lp) lc). rewrite Hd. clear Hd.
+generalize (decompose_correct vars nil (le ++ lp) lc).
+destruct decompose as [lp'|] ; [ |easy].
 assert ((forall (vars0 : list R) (n : nat),
  eval (nth n lc (Econst (Int 0))) vars0 = eval (nth n lc (Econst (Int 0))) nil) /\
  forall k : nat, k < length le ->
@@ -474,47 +495,48 @@ assert ((forall (vars0 : list R) (n : nat),
    (map (fun c : expr => eval c (vars ++ map (fun c0 : expr => eval c0 nil) lc))
         (le ++ lp) ++ vars ++ map (fun c : expr => eval c nil) lc)) 0%R =
  eval (nth k le (Econst (Int 0))) vars) as [H1 H2].
-
-2: { intros H. apply H in H1. clear H.
-     unfold eval_real_nth. now rewrite H1. }
-
+2: { intros H. apply H in H1. unfold eval_real_nth. now rewrite H1. }
 revert lp lc Hf lp'.
-unfold eval_real_nth.
-induction le.
-{ intros lp lc [= <- <-]. split; [ | easy]. now intros vars0 [| n]. }
-intros lp lc. simpl fold_split.
-
-simpl in Ha. apply andb_prop in Ha. destruct Ha as [Ha1 Ha2].
-
-destruct fold_split as (lp0, lc0) eqn:Hf'. intros Hf lp'.
-destruct (IHle Ha2 lp0 lc0 eq_refl lp') as [IH1 IH2]. clear IHle.
-
-generalize (fun v => split_expr_correct v a lp0 lc0). intros Hs.
-destruct split_expr as [ | lp1 lc1] eqn:Hs'; injection Hf as <- <-; split.
-- intros vars0 n. now apply eval_nth_rcons_unique; [apply Hs |].
-- intros [ | k] Hk; simpl in *.
-  { rewrite Hs; [| apply IH1]. now rewrite (Hs vars); [| apply IH1]. }
-  apply lt_S_n in Hk. generalize Hk.
-  intros Hk''. apply IH2 in Hk''. destruct (rcons_unique_correct a lc0) as [l' Hr].
-  rewrite Hr. set (f := fun c : expr =>
-    eval c (vars ++ map (fun c0 : expr => eval c0 nil) (lc0 ++ l'))).
-  change 0%R with (f (Econst (Int 0))). generalize Hk. intros Hk'.
-  apply Nat.lt_le_trans with (2 := (le_plus_l _ (length lp0))) in Hk'.
-  rewrite <-app_length in Hk'. rewrite <-(map_length f) in Hk'.
-  rewrite app_nth1; [ | assumption]. rewrite (map_nth _ _ _ k).
-  rewrite app_nth1; [ | assumption]. unfold f.
-  apply max_arity_correct with (length vars); [ | reflexivity].
+induction le ; intros lp lc.
+{ intros [= <- <-].
+  split ; [ |easy].
+  now intros vars0 [|n]. }
+simpl fold_split.
+simpl in Ha.
+apply andb_prop in Ha.
+destruct Ha as [Ha1 Ha2].
+destruct fold_split as (lp0, lc0) eqn:Hf'.
+intros Hf lp'.
+destruct (IHle Ha2 lp0 lc0 eq_refl lp') as [IH1 _]. clear IHle.
+generalize (fun v => split_expr_correct (Econst (Int 0)) v nil a lp0 lc0).
+intros Hs.
+destruct split_expr as [|lp1 lc1] ; injection Hf as <- <- ; split.
+- intros vars0 n.
+  apply eval_nth_rcons_unique.
+  now apply Hs.
+  easy.
+- intros [|k] Hk ; simpl.
+  { now apply max_arity_correct. }
+  destruct (rcons_unique_correct a lc0) as [l' ->].
+  simpl in Hk.
+  apply lt_S_n in Hk.
+  rewrite app_nth1.
+  2: { rewrite map_length, app_length. lia. }
+  rewrite map_nth with (d := Econst (Int 0)).
+  rewrite app_nth1 by easy.
+  apply max_arity_correct.
   now apply max_arity_nth.
-- intros vars0. now apply Hs.
-- intros [ | k] Hk; simpl in *; [now apply max_arity_correct with (length vars) | ].
-  apply lt_S_n in Hk. set (f := fun c : expr =>
-    eval c (vars ++ map (fun c0 : expr => eval c0 nil) lc1)).
-  change 0%R with (f (Econst (Int 0))). generalize Hk. intros Hk'.
-  apply Nat.lt_le_trans with (2 := (le_plus_l _ (length lp1))) in Hk'.
-  rewrite <-app_length in Hk'. rewrite <-(map_length f) in Hk'.
-  rewrite app_nth1; [ | assumption]. rewrite (map_nth _ _ _ k).
-  rewrite app_nth1; [ | assumption]. unfold f.
-  apply max_arity_correct with (length vars); [ | reflexivity].
+- intros vars0.
+  now apply Hs.
+- intros [|k] Hk ; simpl.
+  { now apply max_arity_correct. }
+  simpl in Hk.
+  apply lt_S_n in Hk.
+  rewrite app_nth1.
+  2: { rewrite map_length, app_length. lia. }
+  rewrite map_nth with (d := Econst (Int 0)).
+  rewrite app_nth1 by easy.
+  apply max_arity_correct.
   now apply max_arity_nth.
 Qed.
 
@@ -537,4 +559,3 @@ generalize (extract_list_correct (e :: nil) vars).
 destruct extract_list; [easy | ]. intros H.
 now specialize (H O (lt_O_Sn _)).
 Qed.
-
